checker/theories/Conversion.v
@@ -1,0 +1,248 @@
+(* Distributed under the terms of the MIT license.   *)
+
+From Coq Require Import Bool String List Program BinPos Compare_dec Arith Lia.
+
+From MetaCoq.Template Require Import config utils Ast AstUtils Induction LiftSubst UnivSubst EnvironmentTyping.
+From MetaCoq.Checker Require Import LibHypsNaming Reflect Reduction.
+
+From Equations Require Import Equations.
+Require Import Equations.Prop.DepElim.
+Require Import ssreflect.
+
+(* Type-valued relations. *)
+Require Import CRelationClasses.
+
+Local Open Scope string_scope.
+Set Asymmetric Patterns.
+
+(** ** Term equality and cumulativity *)
+
+(* ** Syntactic equality up-to universes
+
+  We shouldn't look at printing annotations nor casts.
+  It is however not possible to write a structurally recursive definition
+  for syntactic equality up-to casts due to the [tApp (tCast f _ _) args] case.
+  We hence implement first an equality which considers casts and do a stripping
+  phase of casts before checking equality. *)
+
+
+Inductive eq_term_upto_univ (Re Rle : universe -> universe -> Prop) : term -> term -> Prop :=
+| eq_Rel n  :
+    eq_term_upto_univ Re Rle (tRel n) (tRel n)
+
+| eq_Evar e args args' :
+    Forall2 (eq_term_upto_univ Re Re) args args' ->
+    eq_term_upto_univ Re Rle (tEvar e args) (tEvar e args')
+
+| eq_Var id :
+    eq_term_upto_univ Re Rle (tVar id) (tVar id)
+
+| eq_Sort s s' :
+    Rle s s' ->
+    eq_term_upto_univ Re Rle (tSort s) (tSort s')
+
+| eq_Cast f f' k T T' :
+    eq_term_upto_univ Re Re f f' ->
+    eq_term_upto_univ Re Re T T' ->
+    eq_term_upto_univ Re Rle (tCast f k T) (tCast f' k T')
+
+| eq_App t t' args args' :
+    eq_term_upto_univ Re Rle t t' ->
+    Forall2 (eq_term_upto_univ Re Re) args args' ->
+    eq_term_upto_univ Re Rle (tApp t args) (tApp t' args')
+
+| eq_Const c u u' :
+    Forall2 Rle (List.map Universe.make u) (List.map Universe.make u') ->
+    eq_term_upto_univ Re Rle (tConst c u) (tConst c u')
+
+| eq_Ind i u u' :
+    Forall2 Rle (List.map Universe.make u) (List.map Universe.make u') ->
+    eq_term_upto_univ Re Rle (tInd i u) (tInd i u')
+
+| eq_Construct i k u u' :
+    Forall2 Rle (List.map Universe.make u) (List.map Universe.make u') ->
+    eq_term_upto_univ Re Rle (tConstruct i k u) (tConstruct i k u')
+
+| eq_Lambda na na' ty ty' t t' :
+    eq_term_upto_univ Re Re ty ty' ->
+    eq_term_upto_univ Re Rle t t' ->
+    eq_term_upto_univ Re Rle (tLambda na ty t) (tLambda na' ty' t')
+
+| eq_Prod na na' a a' b b' :
+    eq_term_upto_univ Re Re a a' ->
+    eq_term_upto_univ Re Rle b b' ->
+    eq_term_upto_univ Re Rle (tProd na a b) (tProd na' a' b')
+
+| eq_LetIn na na' ty ty' t t' u u' :
+    eq_term_upto_univ Re Re ty ty' ->
+    eq_term_upto_univ Re Re t t' ->
+    eq_term_upto_univ Re Rle u u' ->
+    eq_term_upto_univ Re Rle (tLetIn na ty t u) (tLetIn na' ty' t' u')
+
+| eq_Case ind par p p' c c' brs brs' :
+    eq_term_upto_univ Re Re p p' ->
+    eq_term_upto_univ Re Re c c' ->
+    Forall2 (fun x y =>
+      fst x = fst y /\
+      eq_term_upto_univ Re Re (snd x) (snd y)
+    ) brs brs' ->
+    eq_term_upto_univ Re Rle (tCase (ind, par) p c brs) (tCase (ind, par) p' c' brs')
+
+| eq_Proj p c c' :
+    eq_term_upto_univ Re Re c c' ->
+    eq_term_upto_univ Re Rle (tProj p c) (tProj p c')
+
+| eq_Fix mfix mfix' idx :
+    Forall2 (fun x y =>
+      eq_term_upto_univ Re Re x.(dtype) y.(dtype) /\
+      eq_term_upto_univ Re Re x.(dbody) y.(dbody) /\
+      x.(rarg) = y.(rarg)
+    ) mfix mfix' ->
+    eq_term_upto_univ Re Rle (tFix mfix idx) (tFix mfix' idx)
+
+| eq_CoFix mfix mfix' idx :
+    Forall2 (fun x y =>
+      eq_term_upto_univ Re Re x.(dtype) y.(dtype) /\
+      eq_term_upto_univ Re Re x.(dbody) y.(dbody) /\
+      x.(rarg) = y.(rarg)
+    ) mfix mfix' ->
+    eq_term_upto_univ Re Rle (tCoFix mfix idx) (tCoFix mfix' idx).
+
+Definition eq_term `{checker_flags} φ :=
+  eq_term_upto_univ (eq_universe φ) (eq_universe φ).
+
+(* ** Syntactic cumulativity up-to universes
+
+  We shouldn't look at printing annotations *)
+
+Definition leq_term `{checker_flags} φ :=
+  eq_term_upto_univ (eq_universe φ) (leq_universe φ).
+
+Fixpoint strip_casts t :=
+  match t with
+  | tEvar ev args => tEvar ev (List.map strip_casts args)
+  | tLambda na T M => tLambda na (strip_casts T) (strip_casts M)
+  | tApp u v => mkApps (strip_casts u) (List.map (strip_casts) v)
+  | tProd na A B => tProd na (strip_casts A) (strip_casts B)
+  | tCast c kind t => strip_casts c
+  | tLetIn na b t b' => tLetIn na (strip_casts b) (strip_casts t) (strip_casts b')
+  | tCase ind p c brs =>
+    let brs' := List.map (on_snd (strip_casts)) brs in
+    tCase ind (strip_casts p) (strip_casts c) brs'
+  | tProj p c => tProj p (strip_casts c)
+  | tFix mfix idx =>
+    let mfix' := List.map (map_def strip_casts strip_casts) mfix in
+    tFix mfix' idx
+  | tCoFix mfix idx =>
+    let mfix' := List.map (map_def strip_casts strip_casts) mfix in
+    tCoFix mfix' idx
+  | tRel _ | tVar _ | tSort _ | tConst _ _ | tInd _ _ | tConstruct _ _ _ => t
+  end.
+
+Definition eq_term_nocast `{checker_flags} (φ : constraints) (t u : term) :=
+  eq_term φ (strip_casts t) (strip_casts u).
+
+Definition leq_term_nocast `{checker_flags} (φ : constraints) (t u : term) :=
+  leq_term φ (strip_casts t) (strip_casts u).
+
+(** ** Cumulativity and Conversion ** *)
+
+Reserved Notation " Σ ;;; Γ |- t <= u " (at level 50, Γ, t, u at next level).
+Reserved Notation " Σ ;;; Γ |- t = u " (at level 50, Γ, t, u at next level).
+
+Inductive cumul `{checker_flags} (Σ : global_env_ext) (Γ : context) : term -> term -> Type :=
+| cumul_refl t u : leq_term (global_ext_constraints Σ) t u -> Σ ;;; Γ |- t <= u
+| cumul_red_l t u v : red1 Σ.1 Γ t v -> Σ ;;; Γ |- v <= u -> Σ ;;; Γ |- t <= u
+| cumul_red_r t u v : Σ ;;; Γ |- t <= v -> red1 Σ.1 Γ u v -> Σ ;;; Γ |- t <= u
+where " Σ ;;; Γ |- t <= u " := (cumul Σ Γ t u) : type_scope.
+
+
+Inductive conv `{checker_flags} (Σ : global_env_ext) (Γ : context) : term -> term -> Type :=
+| conv_refl t u : eq_term (global_ext_constraints Σ) t u -> Σ ;;; Γ |- t = u
+| conv_red_l t u v : red1 Σ Γ t v -> Σ ;;; Γ |- v = u -> Σ ;;; Γ |- t = u
+| conv_red_r t u v : Σ ;;; Γ |- t = v -> red1 (fst Σ) Γ u v -> Σ ;;; Γ |- t = u
+where " Σ ;;; Γ |- t = u " := (@conv _ Σ Γ t u) : type_scope.
+
+
+Lemma cumul_alt {cf:checker_flags} Σ Γ t u :
+  Σ ;;; Γ |- t <= u <~> ∑ v v', red Σ Γ t v × red Σ Γ u v' × leq_term Σ v v'.
+Proof.
+  split.
+  { induction 1. exists t, u. intuition auto; constructor.
+    destruct IHX as (v' & v'' & redv & redv' & leqv).
+    exists v', v''. intuition auto. now eapply red_step.
+    destruct IHX as (v' & v'' & redv & redv' & leqv).
+    exists v', v''. intuition auto. now eapply red_step. }
+  { intros [v [v' [redv [redv' Hleq]]]]. apply red_alt in redv.
+    apply red_alt in redv'.
+    apply clos_rt_rt1n in redv.
+    apply clos_rt_rt1n in redv'.
+    induction redv. induction redv'. constructor; auto.
+    econstructor 3; eauto.
+    econstructor 2; eauto. }
+Qed.
+
+
+Lemma conv_alt {cf:checker_flags} Σ Γ t u :
+  Σ ;;; Γ |- t = u <~> ∑ v v', red Σ Γ t v × red Σ Γ u v' × eq_term Σ v v'.
+Proof.
+  split.
+  { induction 1. exists t, u. intuition auto; constructor.
+    destruct IHX as (v' & v'' & redv & redv' & leqv).
+    exists v', v''. intuition auto. now eapply red_step.
+    destruct IHX as (v' & v'' & redv & redv' & leqv).
+    exists v', v''. intuition auto. now eapply red_step. }
+  { intros [v [v' [redv [redv' Hleq]]]]. apply red_alt in redv.
+    apply red_alt in redv'.
+    apply clos_rt_rt1n in redv.
+    apply clos_rt_rt1n in redv'.
+    induction redv. induction redv'. constructor; auto.
+    econstructor 3; eauto.
+    econstructor 2; eauto. }
+Qed.
+
+
+
+
+(** ** Context conversion ** *)
+
+Inductive context_relation
+          (P : context -> context -> context_decl -> context_decl -> Type)
+          : forall (Γ Γ' : context), Type :=
+| ctx_rel_nil : context_relation P nil nil
+| ctx_rel_vass na na' T U Γ Γ' :
+    context_relation P Γ Γ' ->
+    P Γ Γ' (vass na T) (vass na' U) ->
+    context_relation P (vass na T :: Γ) (vass na' U :: Γ')
+| ctx_rel_def na na' t T u U Γ Γ' :
+    context_relation P Γ Γ' ->
+    P Γ Γ' (vdef na t T) (vdef na' u U) ->
+    context_relation P (vdef na t T :: Γ) (vdef na' u U :: Γ').
+Derive Signature for context_relation.
+Arguments context_relation P Γ Γ' : clear implicits.
+
+Section ConvContext.
+
+  Context {cf:checker_flags} (Σ : global_env_ext).
+
+  Inductive conv_decls (Γ Γ' : context) : forall (x y : context_decl), Type :=
+  | conv_vass na na' T T' :
+      (* isType Σ Γ' T' -> *)
+      Σ ;;; Γ |- T = T' ->
+      conv_decls Γ Γ' (vass na T) (vass na' T')
+
+  | conv_vdef_type na na' b T T' :
+      (* isType Σ Γ' T' -> *)
+      Σ ;;; Γ |- T = T' ->
+      conv_decls Γ Γ' (vdef na b T) (vdef na' b T')
+
+  | conv_vdef_body na na' b b' T T' :
+      (* isType Σ Γ' T' -> *)
+      (* Σ ;;; Γ' |- b' : T' -> *)
+      Σ ;;; Γ |- b = b' ->
+      Σ ;;; Γ |- T = T' ->
+      conv_decls Γ Γ' (vdef na b T) (vdef na' b' T').
+
+End ConvContext.
+
+Notation conv_context Σ Γ Γ' := (context_relation (conv_decls Σ) Γ Γ').
