checker/theories/Reduction.v
@@ -1,0 +1,480 @@
+
+From Coq Require Import Bool String List Program BinPos Compare_dec Arith Lia.
+
+From MetaCoq.Template Require Import config utils Ast AstUtils Induction LiftSubst UnivSubst EnvironmentTyping.
+From MetaCoq.Checker Require Import LibHypsNaming Reflect.
+
+From Equations Require Import Equations.
+Require Import Equations.Prop.DepElim.
+Require Import ssreflect.
+
+(* Type-valued relations. *)
+Require Import CRelationClasses.
+
+Local Open Scope string_scope.
+Set Asymmetric Patterns.
+
+Module TemplateLookup := Lookup TemplateTerm TemplateEnvironment.
+Include TemplateLookup.
+
+(** ** Reduction *)
+
+(** *** Helper functions for reduction *)
+
+Definition fix_subst (l : mfixpoint term) :=
+  let fix aux n :=
+      match n with
+      | 0 => []
+      | S n => tFix l n :: aux n
+      end
+  in aux (List.length l).
+
+Definition unfold_fix (mfix : mfixpoint term) (idx : nat) :=
+  match List.nth_error mfix idx with
+  | Some d => Some (d.(rarg), subst0 (fix_subst mfix) d.(dbody))
+  | None => None
+  end.
+
+Definition cofix_subst (l : mfixpoint term) :=
+  let fix aux n :=
+      match n with
+      | 0 => []
+      | S n => tCoFix l n :: aux n
+      end
+  in aux (List.length l).
+
+Definition unfold_cofix (mfix : mfixpoint term) (idx : nat) :=
+  match List.nth_error mfix idx with
+  | Some d => Some (d.(rarg), subst0 (cofix_subst mfix) d.(dbody))
+  | None => None
+  end.
+
+Definition isConstruct_app t :=
+  match fst (decompose_app t) with
+  | tConstruct _ _ _ => true
+  | _ => false
+  end.
+
+Definition is_constructor n ts :=
+  match List.nth_error ts n with
+  | Some a => isConstruct_app a
+  | None => false
+  end.
+
+Lemma fix_subst_length mfix : #|fix_subst mfix| = #|mfix|.
+Proof.
+  unfold fix_subst. generalize (tFix mfix). intros.
+  induction mfix; simpl; auto.
+Qed.
+
+Lemma cofix_subst_length mfix : #|cofix_subst mfix| = #|mfix|.
+Proof.
+  unfold cofix_subst. generalize (tCoFix mfix). intros.
+  induction mfix; simpl; auto.
+Qed.
+
+Definition fix_context (m : mfixpoint term) : context :=
+  List.rev (mapi (fun i d => vass d.(dname) (lift0 i d.(dtype))) m).
+
+Lemma fix_context_length mfix : #|fix_context mfix| = #|mfix|.
+Proof. unfold fix_context. now rewrite List.rev_length mapi_length. Qed.
+
+Definition tDummy := tVar "".
+
+Definition iota_red npar c args brs :=
+  (mkApps (snd (List.nth c brs (0, tDummy))) (List.skipn npar args)).
+
+
+(** *** One step strong beta-zeta-iota-fix-delta reduction
+
+  Inspired by the reduction relation from Coq in Coq [Barras'99].
+*)
+
+Local Open Scope type_scope.
+Arguments OnOne2 {A} P%type l l'.
+
+Inductive red1 (Σ : global_env) (Γ : context) : term -> term -> Type :=
+(** Reductions *)
+(** Beta *)
+| red_beta na t b a l :
+    red1 Σ Γ (tApp (tLambda na t b) (a :: l)) (mkApps (subst10 a b) l)
+
+(** Let *)
+| red_zeta na b t b' :
+    red1 Σ Γ (tLetIn na b t b') (subst10 b b')
+
+| red_rel i body :
+    option_map decl_body (nth_error Γ i) = Some (Some body) ->
+    red1 Σ Γ (tRel i) (lift0 (S i) body)
+
+(** Case *)
+| red_iota ind pars c u args p brs :
+    red1 Σ Γ (tCase (ind, pars) p (mkApps (tConstruct ind c u) args) brs)
+         (iota_red pars c args brs)
+
+(** Fix unfolding, with guard *)
+| red_fix mfix idx args narg fn :
+    unfold_fix mfix idx = Some (narg, fn) ->
+    is_constructor narg args = true ->
+    red1 Σ Γ (tApp (tFix mfix idx) args) (tApp fn args)
+
+(** CoFix-case unfolding *)
+| red_cofix_case ip p mfix idx args narg fn brs :
+    unfold_cofix mfix idx = Some (narg, fn) ->
+    red1 Σ Γ (tCase ip p (mkApps (tCoFix mfix idx) args) brs)
+         (tCase ip p (mkApps fn args) brs)
+
+(** CoFix-proj unfolding *)
+| red_cofix_proj p mfix idx args narg fn :
+    unfold_cofix mfix idx = Some (narg, fn) ->
+    red1 Σ Γ (tProj p (mkApps (tCoFix mfix idx) args))
+         (tProj p (mkApps fn args))
+(* FIXME: We should really be dual to Fix: ask directly
+   for the constructor, applied, and project the argument:
+
+    unfold_cofix mfix idx = Some (narg, mkApps (tConstruct ind c u) args') ->
+    nth_error args' (pars + narg) = Some arg ->
+    red1 Σ Γ (tProj (i, pars, narg) (mkApps (tCoFix mfix idx) args))
+             (mkApps arg args)
+
+    Otherwise confluence fails, AFAICT.
+
+    (tProj (i, pars, narg) (mkApps fn args))
+*)
+(** Constant unfolding *)
+| red_delta c decl body (isdecl : declared_constant Σ c decl) u :
+    decl.(cst_body) = Some body ->
+    red1 Σ Γ (tConst c u) (subst_instance_constr u body)
+
+(** Proj *)
+| red_proj i pars narg args k u arg:
+    nth_error args (pars + narg) = Some arg ->
+    red1 Σ Γ (tProj (i, pars, narg) (mkApps (tConstruct i k u) args)) arg
+
+
+| abs_red_l na M M' N : red1 Σ Γ M M' -> red1 Σ Γ (tLambda na M N) (tLambda na M' N)
+| abs_red_r na M M' N : red1 Σ (Γ ,, vass na N) M M' -> red1 Σ Γ (tLambda na N M) (tLambda na N M')
+
+| letin_red_def na b t b' r : red1 Σ Γ b r -> red1 Σ Γ (tLetIn na b t b') (tLetIn na r t b')
+| letin_red_ty na b t b' r : red1 Σ Γ t r -> red1 Σ Γ (tLetIn na b t b') (tLetIn na b r b')
+| letin_red_body na b t b' r : red1 Σ (Γ ,, vdef na b t) b' r -> red1 Σ Γ (tLetIn na b t b') (tLetIn na b t r)
+
+| case_red_pred ind p p' c brs : red1 Σ Γ p p' -> red1 Σ Γ (tCase ind p c brs) (tCase ind p' c brs)
+| case_red_discr ind p c c' brs : red1 Σ Γ c c' -> red1 Σ Γ (tCase ind p c brs) (tCase ind p c' brs)
+| case_red_brs ind p c brs brs' : OnOne2 (fun x y => red1 Σ Γ (snd x) (snd y)) brs brs' -> red1 Σ Γ (tCase ind p c brs) (tCase ind p c brs')
+
+| proj_red p c c' : red1 Σ Γ c c' -> red1 Σ Γ (tProj p c) (tProj p c')
+
+| app_red_l M1 N1 M2 : red1 Σ Γ M1 N1 -> red1 Σ Γ (tApp M1 M2) (mkApps N1 M2)
+| app_red_r M2 N2 M1 : OnOne2 (red1 Σ Γ) M2 N2 -> red1 Σ Γ (tApp M1 M2) (tApp M1 N2)
+
+| prod_red_l na M1 M2 N1 : red1 Σ Γ M1 N1 -> red1 Σ Γ (tProd na M1 M2) (tProd na N1 M2)
+| prod_red_r na M2 N2 M1 : red1 Σ (Γ ,, vass na M1) M2 N2 ->
+                               red1 Σ Γ (tProd na M1 M2) (tProd na M1 N2)
+
+| evar_red ev l l' : OnOne2 (red1 Σ Γ) l l' -> red1 Σ Γ (tEvar ev l) (tEvar ev l')
+
+| cast_red_l M1 k M2 N1 : red1 Σ Γ M1 N1 -> red1 Σ Γ (tCast M1 k M2) (tCast N1 k M2)
+| cast_red_r M2 k N2 M1 : red1 Σ Γ M2 N2 -> red1 Σ Γ (tCast M1 k M2) (tCast M1 k N2)
+| cast_red M1 k M2 : red1 Σ Γ (tCast M1 k M2) M1
+
+| fix_red_ty mfix0 mfix1 idx :
+    OnOne2 (fun d0 d1 => red1 Σ Γ (dtype d0) (dtype d1) * (dbody d0 = dbody d1))%type mfix0 mfix1 ->
+    red1 Σ Γ (tFix mfix0 idx) (tFix mfix1 idx)
+
+| fix_red_body mfix0 mfix1 idx :
+    OnOne2 (fun d0 d1 => red1 Σ (Γ ,,, fix_context mfix0) (dbody d0) (dbody d1) * (dtype d0 = dtype d1))
+           mfix0 mfix1 ->
+    red1 Σ Γ (tFix mfix0 idx) (tFix mfix1 idx)
+
+| cofix_red_ty mfix0 mfix1 idx :
+    OnOne2 (fun d0 d1 => red1 Σ Γ (dtype d0) (dtype d1) * (dbody d0 = dbody d1))%type mfix0 mfix1 ->
+    red1 Σ Γ (tCoFix mfix0 idx) (tCoFix mfix1 idx)
+
+| cofix_red_body mfix0 mfix1 idx :
+    OnOne2 (fun d0 d1 => red1 Σ (Γ ,,, fix_context mfix0) (dbody d0) (dbody d1) * (dtype d0 = dtype d1))%type mfix0 mfix1 ->
+    red1 Σ Γ (tCoFix mfix0 idx) (tCoFix mfix1 idx).
+
+Lemma red1_ind_all :
+  forall (Σ : global_env) (P : context -> term -> term -> Type),
+       (forall (Γ : context) (na : name) (t b a : term) (l : list term),
+        P Γ (tApp (tLambda na t b) (a :: l)) (mkApps (b {0 := a}) l)) ->
+       (forall (Γ : context) (na : name) (b t b' : term), P Γ (tLetIn na b t b') (b' {0 := b})) ->
+
+       (forall (Γ : context) (i : nat) (body : term),
+        option_map decl_body (nth_error Γ i) = Some (Some body) -> P Γ (tRel i) ((lift0 (S i)) body)) ->
+
+       (forall (Γ : context) (ind : inductive) (pars c : nat) (u : universe_instance) (args : list term)
+          (p : term) (brs : list (nat * term)),
+        P Γ (tCase (ind, pars) p (mkApps (tConstruct ind c u) args) brs) (iota_red pars c args brs)) ->
+
+       (forall (Γ : context) (mfix : mfixpoint term) (idx : nat) (args : list term) (narg : nat) (fn : term),
+        unfold_fix mfix idx = Some (narg, fn) ->
+        is_constructor narg args = true -> P Γ (tApp (tFix mfix idx) args) (tApp fn args)) ->
+       (forall (Γ : context) (ip : inductive * nat) (p : term) (mfix : mfixpoint term) (idx : nat)
+          (args : list term) (narg : nat) (fn : term) (brs : list (nat * term)),
+        unfold_cofix mfix idx = Some (narg, fn) ->
+        P Γ (tCase ip p (mkApps (tCoFix mfix idx) args) brs) (tCase ip p (mkApps fn args) brs)) ->
+
+       (forall (Γ : context) (p : projection) (mfix : mfixpoint term) (idx : nat) (args : list term)
+          (narg : nat) (fn : term),
+        unfold_cofix mfix idx = Some (narg, fn) -> P Γ (tProj p (mkApps (tCoFix mfix idx) args)) (tProj p (mkApps fn args))) ->
+
+       (forall (Γ : context) (c : ident) (decl : constant_body) (body : term),
+        declared_constant Σ c decl ->
+        forall u : universe_instance, cst_body decl = Some body -> P Γ (tConst c u) (subst_instance_constr u body)) ->
+
+       (forall (Γ : context) (i : inductive) (pars narg : nat) (args : list term) (k : nat) (u : universe_instance)
+         (arg : term),
+           nth_error args (pars + narg) = Some arg ->
+           P Γ (tProj (i, pars, narg) (mkApps (tConstruct i k u) args)) arg) ->
+
+       (forall (Γ : context) (na : name) (M M' N : term),
+        red1 Σ Γ M M' -> P Γ M M' -> P Γ (tLambda na M N) (tLambda na M' N)) ->
+
+       (forall (Γ : context) (na : name) (M M' N : term),
+        red1 Σ (Γ,, vass na N) M M' -> P (Γ,, vass na N) M M' -> P Γ (tLambda na N M) (tLambda na N M')) ->
+
+       (forall (Γ : context) (na : name) (b t b' r : term),
+        red1 Σ Γ b r -> P Γ b r -> P Γ (tLetIn na b t b') (tLetIn na r t b')) ->
+
+       (forall (Γ : context) (na : name) (b t b' r : term),
+        red1 Σ Γ t r -> P Γ t r -> P Γ (tLetIn na b t b') (tLetIn na b r b')) ->
+
+       (forall (Γ : context) (na : name) (b t b' r : term),
+        red1 Σ (Γ,, vdef na b t) b' r -> P (Γ,, vdef na b t) b' r -> P Γ (tLetIn na b t b') (tLetIn na b t r)) ->
+
+       (forall (Γ : context) (ind : inductive * nat) (p p' c : term) (brs : list (nat * term)),
+        red1 Σ Γ p p' -> P Γ p p' -> P Γ (tCase ind p c brs) (tCase ind p' c brs)) ->
+
+       (forall (Γ : context) (ind : inductive * nat) (p c c' : term) (brs : list (nat * term)),
+        red1 Σ Γ c c' -> P Γ c c' -> P Γ (tCase ind p c brs) (tCase ind p c' brs)) ->
+
+       (forall (Γ : context) (ind : inductive * nat) (p c : term) (brs brs' : list (nat * term)),
+           OnOne2 (fun x y : nat * term => red1 Σ Γ (snd x) (snd y) * P Γ (snd x) (snd y)) brs brs' ->
+           P Γ (tCase ind p c brs) (tCase ind p c brs')) ->
+
+       (forall (Γ : context) (p : projection) (c c' : term), red1 Σ Γ c c' -> P Γ c c' -> P Γ (tProj p c) (tProj p c')) ->
+
+       (forall (Γ : context) (M1 N1 : term) (M2 : list term), red1 Σ Γ M1 N1 -> P Γ M1 N1 -> P Γ (tApp M1 M2) (mkApps N1 M2)) ->
+
+       (forall (Γ : context) (M2 N2 : list term) (M1 : term), OnOne2 (fun x y => red1 Σ Γ x y * P Γ x y)%type M2 N2 -> P Γ (tApp M1 M2) (tApp M1 N2)) ->
+
+       (forall (Γ : context) (na : name) (M1 M2 N1 : term),
+        red1 Σ Γ M1 N1 -> P Γ M1 N1 -> P Γ (tProd na M1 M2) (tProd na N1 M2)) ->
+
+       (forall (Γ : context) (na : name) (M2 N2 M1 : term),
+        red1 Σ (Γ,, vass na M1) M2 N2 -> P (Γ,, vass na M1) M2 N2 -> P Γ (tProd na M1 M2) (tProd na M1 N2)) ->
+
+       (forall (Γ : context) (ev : nat) (l l' : list term), OnOne2 (fun x y => red1 Σ Γ x y * P Γ x y) l l' -> P Γ (tEvar ev l) (tEvar ev l')) ->
+
+       (forall (Γ : context) (M1 : term) (k : cast_kind) (M2 N1 : term),
+        red1 Σ Γ M1 N1 -> P Γ M1 N1 -> P Γ (tCast M1 k M2) (tCast N1 k M2)) ->
+
+       (forall (Γ : context) (M2 : term) (k : cast_kind) (N2 M1 : term),
+        red1 Σ Γ M2 N2 -> P Γ M2 N2 -> P Γ (tCast M1 k M2) (tCast M1 k N2)) ->
+
+       (forall (Γ : context) (M1 : term) (k : cast_kind) (M2 : term),
+           P Γ (tCast M1 k M2) M1) ->
+
+       (forall (Γ : context) (mfix0 mfix1 : list (def term)) (idx : nat),
+        OnOne2 (fun d0 d1 : def term => red1 Σ Γ (dtype d0) (dtype d1) * (dbody d0 = dbody d1) * P Γ (dtype d0) (dtype d1)) mfix0 mfix1 ->
+        P Γ (tFix mfix0 idx) (tFix mfix1 idx)) ->
+
+       (forall (Γ : context) (mfix0 mfix1 : list (def term)) (idx : nat),
+        OnOne2 (fun d0 d1 : def term =>
+                  red1 Σ (Γ ,,, fix_context mfix0) (dbody d0) (dbody d1) * (dtype d0 = dtype d1) *
+                  P (Γ ,,, fix_context mfix0) (dbody d0) (dbody d1)) mfix0 mfix1 ->
+        P Γ (tFix mfix0 idx) (tFix mfix1 idx)) ->
+
+       (forall (Γ : context) (mfix0 mfix1 : list (def term)) (idx : nat),
+        OnOne2 (fun d0 d1 : def term => red1 Σ Γ (dtype d0) (dtype d1) * (dbody d0 = dbody d1) *
+                                        P Γ (dtype d0) (dtype d1)) mfix0 mfix1 ->
+        P Γ (tCoFix mfix0 idx) (tCoFix mfix1 idx)) ->
+
+       (forall (Γ : context) (mfix0 mfix1 : list (def term)) (idx : nat),
+        OnOne2 (fun d0 d1 : def term => red1 Σ (Γ ,,, fix_context mfix0) (dbody d0) (dbody d1) * (dtype d0 = dtype d1) * P (Γ ,,, fix_context mfix0) (dbody d0) (dbody d1)) mfix0 mfix1 ->
+        P Γ (tCoFix mfix0 idx) (tCoFix mfix1 idx)) ->
+
+       forall (Γ : context) (t t0 : term), red1 Σ Γ t t0 -> P Γ t t0.
+Proof.
+  intros. rename X29 into Xlast. revert Γ t t0 Xlast.
+  fix aux 4. intros Γ t T.
+  move aux at top.
+  destruct 1; match goal with
+              | |- P _ (tFix _ _) (tFix _ _) => idtac
+              | |- P _ (tCoFix _ _) (tCoFix _ _) => idtac
+              | |- P _ (tApp (tFix _ _) _) _ => idtac
+              | |- P _ (tCase _ _ (mkApps (tCoFix _ _) _) _) _ => idtac
+              | |- P _ (tProj _ (mkApps (tCoFix _ _) _)) _ => idtac
+              | H : _ |- _ => eapply H; eauto
+              end.
+  - eapply X3; eauto.
+  - eapply X4; eauto.
+  - eapply X5; eauto.
+
+  - revert brs brs' o.
+    fix auxl 3.
+    intros l l' Hl. destruct Hl.
+    constructor. split; auto.
+    constructor. auto.
+
+  - revert M2 N2 o.
+    fix auxl 3.
+    intros l l' Hl. destruct Hl.
+    constructor. split; auto.
+    constructor. auto.
+
+  - revert l l' o.
+    fix auxl 3.
+    intros l l' Hl. destruct Hl.
+    constructor. split; auto.
+    constructor. auto.
+
+  - eapply X25.
+    revert mfix0 mfix1 o; fix auxl 3; intros l l' Hl; destruct Hl;
+      constructor; try split; auto; intuition.
+
+  - eapply X26.
+    revert o. generalize (fix_context mfix0). intros c H28.
+    revert mfix0 mfix1 H28; fix auxl 3; intros l l' Hl;
+    destruct Hl; constructor; try split; auto; intuition.
+
+  - eapply X27.
+    revert mfix0 mfix1 o; fix auxl 3; intros l l' Hl; destruct Hl;
+      constructor; try split; auto; intuition.
+
+  - eapply X28.
+    revert o. generalize (fix_context mfix0). intros c H28.
+    revert mfix0 mfix1 H28; fix auxl 3; intros l l' Hl; destruct Hl;
+      constructor; try split; auto; intuition.
+Defined.
+
+(** *** Reduction
+
+  The reflexive-transitive closure of 1-step reduction. *)
+
+Inductive red Σ Γ M : term -> Type :=
+| refl_red : red Σ Γ M M
+| trans_red : forall (P : term) N, red Σ Γ M P -> red1 Σ Γ P N -> red Σ Γ M N.
+
+
+(** Simple lemmas about reduction *)
+
+Lemma red1_red (Σ : global_env) Γ t u : red1 Σ Γ t u -> red Σ Γ t u.
+Proof. econstructor; eauto. constructor. Qed.
+Hint Resolve red1_red refl_red.
+
+Lemma red_step Σ Γ t u v : red1 Σ Γ t u -> red Σ Γ u v -> red Σ Γ t v.
+Proof.
+  induction 2. econstructor; auto.
+  econstructor 2; eauto.
+Qed.
+
+
+(* I can't reuse Equations' one because of an extraction bug ? *)
+
+Section Reflexive_Transitive_Closure.
+  Context {A : Type} (R : crelation A).
+
+  (** Definition by direct reflexive-transitive closure *)
+
+  Inductive clos_refl_trans (x:A) : A -> Type :=
+  | rt_step (y:A) : R x y -> clos_refl_trans x y
+  | rt_refl : clos_refl_trans x x
+  | rt_trans (y z:A) :
+      clos_refl_trans x y -> clos_refl_trans y z -> clos_refl_trans x z.
+
+  (** Alternative definition by transitive extension on the left *)
+
+  Inductive clos_refl_trans_1n (x: A) : A -> Type :=
+  | rt1n_refl : clos_refl_trans_1n x x
+  | rt1n_trans (y z:A) :
+      R x y -> clos_refl_trans_1n y z -> clos_refl_trans_1n x z.
+
+  (** Alternative definition by transitive extension on the right *)
+
+  Inductive clos_refl_trans_n1 (x: A) : A -> Type :=
+  | rtn1_refl : clos_refl_trans_n1 x x
+  | rtn1_trans (y z:A) :
+      R y z -> clos_refl_trans_n1 x y -> clos_refl_trans_n1 x z.
+
+  Lemma clos_rt1n_rt : forall x y,
+      clos_refl_trans_1n x y -> clos_refl_trans x y.
+  Proof.
+    induction 1.
+    constructor 2.
+    constructor 3 with y; auto.
+    constructor 1; auto.
+  Qed.
+
+  Lemma clos_rt1n_step : forall x y, R x y -> clos_refl_trans_1n x y.
+  Proof.
+    intros x y H.
+    right with y;[assumption|left].
+  Qed.
+
+  Lemma clos_rt_rt1n : forall x y,
+      clos_refl_trans x y -> clos_refl_trans_1n x y.
+  Proof.
+    induction 1.
+    apply clos_rt1n_step; assumption.
+    left.
+    generalize IHX2; clear IHX2;
+      induction IHX1; auto.
+
+    right with y; auto.
+    eapply IHIHX1; auto.
+    apply clos_rt1n_rt; auto.
+  Qed.
+
+
+  Lemma clos_rtn1_rt : forall x y,
+      clos_refl_trans_n1 x y -> clos_refl_trans x y.
+  Proof.
+    induction 1.
+    constructor 2.
+    constructor 3 with y; auto.
+    constructor 1; assumption.
+  Qed.
+
+  Lemma clos_rtn1_step : forall x y, R x y -> clos_refl_trans_n1 x y.
+  Proof.
+    intros x y H.
+    right with x;[assumption|left].
+  Qed.
+
+  Lemma clos_rt_rtn1 :  forall x y,
+      clos_refl_trans x y -> clos_refl_trans_n1 x y.
+  Proof.
+    induction 1.
+    apply clos_rtn1_step; auto.
+    left.
+    elim IHX2; auto.
+    intros.
+    right with y0; auto.
+  Qed.
+
+End Reflexive_Transitive_Closure.
+
+Lemma red_alt Σ Γ t u : red Σ Γ t u <~> clos_refl_trans (red1 Σ Γ) t u.
+Proof.
+  split.
+  - intros H. apply clos_rtn1_rt.
+    induction H. constructor.
+    econstructor; tea.
+  - intros H. apply clos_rt_rtn1 in H.
+    induction H; econstructor; eauto.
+Qed.
+
+
+Lemma red_trans Σ Γ t u v : red Σ Γ t u -> red Σ Γ u v -> red Σ Γ t v.
+Proof.
+  intros. apply red_alt. apply red_alt in X. apply red_alt in X0. now econstructor 3.
+Defined.
+
+Instance red_Transitive Σ Γ : Transitive (red Σ Γ).
+Proof. refine (red_trans _ _). Qed.
+
+Instance red_Reflexive Σ Γ : Reflexive (red Σ Γ)
+  := refl_red _ _.
