checker/theories/TypingWf.v
@@ -430,7 +430,7 @@ Proof.
     apply wf_subst; auto with wf. apply wf_subst_instance_constr.
     eapply declared_constructor_wf; eauto.
   - split. wf. constructor; eauto. solve_all.
-    apply wf_mkApps. wf. solve_all. apply wf_mkApps_inv in H7. solve_all.
+    apply wf_mkApps. wf. solve_all. apply wf_mkApps_inv in H6. solve_all.
     apply All_app_inv; solve_all. now apply All_skipn.
   - split. wf. apply wf_subst. solve_all. constructor. wf.
     apply wf_mkApps_inv in H2. apply All_rev. solve_all.
