checker/theories/WeakeningEnv.v
@@ -276,12 +276,11 @@ Proof.
   eapply eq_decl_subset; eassumption. assumption.
 Qed.
 
-Lemma check_correct_arity_subset {cf:checker_flags} φ φ' decl ind u ctx pars pctx
-  : ConstraintSet.Subset φ φ' -> check_correct_arity φ decl ind u ctx pars pctx
-    -> check_correct_arity φ' decl ind u ctx pars pctx.
+Lemma check_correct_arity_extends {cf:checker_flags} Σ Σ' φ decl ind u ctx pars pctx
+  : extends Σ Σ' -> check_correct_arity (Σ, φ) decl ind u ctx pars pctx
+    -> check_correct_arity (Σ', φ) decl ind u ctx pars pctx.
 Proof.
-  apply eq_context_subset.
-Qed.
+Admitted.
 
 Lemma weakening_env_consistent_instance {cf:checker_flags} :
   forall Σ Σ' φ ctrs u,
@@ -325,8 +324,7 @@ Proof.
     induction X1. constructor. econstructor; eauto with extends.
     eapply weakening_env_cumul in cumul; eauto.
   - econstructor; eauto 2 with extends.
-    + eapply check_correct_arity_subset; tea.
-      apply weakening_env_global_ext_constraints; tas.
+    + destruct Σ; eapply check_correct_arity_extends; tea.
     + close_Forall. intros; intuition eauto with extends.
   - econstructor; eauto with extends.
     eapply All_local_env_impl. eapply X.
